\begin{proof} $ $\\
$t^2(t-1)^2(t-2)^2(t-3)^2$\\\\
\tikz {
        \path
        (0, 0) node[circle, fill=black] (1) {}
        (2, 0) node[circle, fill=black] (2) {}
        (0, -2) node[circle, fill=black] (3) {}
        (2, -2) node[circle, fill=black] (4) {}

        (4, 0) node[circle, fill=black] (5) {}
        (6, 0) node[circle, fill=black] (6) {}
        (4, -2) node[circle, fill=black] (7) {}
        (6, -2) node[circle, fill=black] (8) {};

        \draw (1) -- (2);
        \draw (1) -- (3);
        \draw (1) -- (4);
        \draw (2) -- (3);
        \draw (2) -- (4);
        \draw (3) -- (4);

        \draw (5) -- (6);
        \draw (5) -- (7);
        \draw (5) -- (8);
        \draw (6) -- (7);
        \draw (6) -- (8);
        \draw (7) -- (8);
        }$ $\\\\\\
$t(t-1)^3$\\\\
\tikz {
        \path
        (0, 0) node[circle, fill=black] (1) {}
        (2, 0) node[circle, fill=black] (2) {}
        (4, 0) node[circle, fill=black] (3) {}
        (6, 0) node[circle, fill=black] (4) {};

        \draw (1) -- (2);
        \draw (2) -- (3);
        \draw (3) -- (4);
        }$ $\\\\\\
$t(t-1)^3(t-2)$\\\\
\tikz {
        \path
        (0, 0) node[circle, fill=black] (1) {}
        (2, 0) node[circle, fill=black] (2) {}
        (4, 0) node[circle, fill=black] (3) {}
        (6, 0) node[circle, fill=black] (4) {}
        (5, -1) node[circle, fill=black] (5) {};

        \draw (1) -- (2);
        \draw (2) -- (3);
        \draw (3) -- (4);
        \draw (3) -- (5);
        \draw (4) -- (5)
        }
\end{proof}